Proved relationship between standard-LR3 and compressed-LR3

General_Luby_Rackoff.thy
@@ -4,20 +4,26 @@ begin
 
 type_synonym whole = \<open>half \<times> half\<close>
 
-definition X :: \<open>whole update \<Rightarrow> (whole \<times> whole \<times> whole \<times> whole \<times> db \<times> db \<times> db) update\<close> where \<open>X = Fst\<close>
-definition X1 :: \<open>whole update \<Rightarrow> (whole \<times> whole \<times> whole \<times> whole \<times> db \<times> db \<times> db) update\<close> where \<open>X1 = Snd o Fst\<close>
-definition X2 :: \<open>whole update \<Rightarrow> (whole \<times> whole \<times> whole \<times> whole \<times> db \<times> db \<times> db) update\<close> where \<open>X2 = Snd o Snd o Fst\<close>
-definition Y :: \<open>whole update \<Rightarrow> (whole \<times> whole \<times> whole \<times> whole \<times> db \<times> db \<times> db) update\<close> where \<open>Y = Snd o Snd o Snd o Fst\<close>
-definition D1 :: \<open>db update \<Rightarrow> (whole \<times> whole \<times> whole \<times> whole \<times> db \<times> db \<times> db) update\<close> where \<open>D1 = Snd o Snd o Snd o Snd o Fst\<close>
-definition D2 :: \<open>db update \<Rightarrow> (whole \<times> whole \<times> whole \<times> whole \<times> db \<times> db \<times> db) update\<close> where \<open>D2 = Snd o Snd o Snd o Snd o Snd o Fst\<close>
-definition D3 :: \<open>db update \<Rightarrow> (whole \<times> whole \<times> whole \<times> whole \<times> db \<times> db \<times> db) update\<close> where \<open>D3 = Snd o Snd o Snd o Snd o Snd o Snd\<close>
+type_synonym state = \<open>whole \<times> whole \<times> whole \<times> whole \<times> db \<times> db \<times> db\<close>
 
-lemma [simp]: \<open>compatible reg_1_3 reg_2_3\<close> \<open>compatible reg_1_3 reg_3_3\<close> \<open>compatible reg_2_3 reg_3_3\<close>
-  \<open>compatible X X1\<close> \<open>compatible X D1\<close> \<open>compatible X1 D1\<close> \<open>compatible X1 X2\<close> \<open>compatible X1 D3\<close>
-  \<open>compatible X2 D3\<close> \<open>compatible X1 D2\<close> \<open>compatible X2 D2\<close> \<open>compatible X2 Y\<close> \<open>compatible Y D3\<close>
-            apply (simp_all add: reg_1_3_def reg_2_3_def reg_3_3_def X_def X1_def D1_def X2_def
-      D2_def D3_def Y_def)
-  by -
+definition X :: \<open>whole update \<Rightarrow> state update\<close> where \<open>X = Fst\<close>
+definition X1 :: \<open>whole update \<Rightarrow> state update\<close> where \<open>X1 = Snd o Fst\<close>
+definition X2 :: \<open>whole update \<Rightarrow> state update\<close> where \<open>X2 = Snd o Snd o Fst\<close>
+definition Y :: \<open>whole update \<Rightarrow> state update\<close> where \<open>Y = Snd o Snd o Snd o Fst\<close>
+definition D1 :: \<open>db update \<Rightarrow> state update\<close> where \<open>D1 = Snd o Snd o Snd o Snd o Fst\<close>
+definition D2 :: \<open>db update \<Rightarrow> state update\<close> where \<open>D2 = Snd o Snd o Snd o Snd o Snd o Fst\<close>
+definition D3 :: \<open>db update \<Rightarrow> state update\<close> where \<open>D3 = Snd o Snd o Snd o Snd o Snd o Snd\<close>
 
+lemma [simp,register]: \<open>mutually compatible (X,X1,X2,Y,D1,D2,D3)\<close>
+  by (auto simp add: X_def X1_def D1_def X2_def D2_def D3_def Y_def)
+
+(* lemma [simp]: \<open>each register (X,X1,X2,Y,D1,D2,D3)\<close>
+  by (auto simp add: X_def X1_def D1_def X2_def D2_def D3_def Y_def) *)
+
+lemma [simp]: \<open>mutually compatible (reg_1_3, reg_2_3, reg_3_3)\<close>
+  by (auto simp add: reg_1_3_def reg_2_3_def reg_3_3_def)
+
+(* lemma [simp]: \<open>each register (reg_1_3, reg_2_3, reg_3_3)\<close>
+  by (auto simp add: reg_1_3_def reg_2_3_def reg_3_3_def) *)
 
 end
