All.thy
@@ -1,0 +1,5 @@
+theory All
+  imports Rel_LR3_Standard_Compressed
+begin
+
+end
