LR3_Compressed.thy
@@ -1,0 +1,14 @@
+theory LR3_Compressed
+  imports Compressed_Oracles.CO_Invariants Misc_Luby_Rackoff General_Luby_Rackoff
+begin
+
+(* U_UP,i, using compressed queries *)
+definition UPc :: \<open>(whole \<times> whole \<times> db) ell2 \<Rightarrow>\<^sub>C\<^sub>L (whole \<times> whole \<times> db) ell2\<close> where \<open>UPc = 
+  (reg_1_3 o Fst; reg_2_3 o Snd) cnot o\<^sub>C\<^sub>L
+  (reg_1_3 o Snd; reg_2_3 o Fst) cnot o\<^sub>C\<^sub>L
+  (reg_1_3 o Fst; (reg_2_3 o Fst; reg_3_3)) query\<close>
+
+definition LR3c where \<open>LR3c =
+  (X;(X1;D1)) UPc o\<^sub>C\<^sub>L (X1;(X2;D2)) UPc o\<^sub>C\<^sub>L (X2;(Y;D3)) UPc o\<^sub>C\<^sub>L (X1;(X2;D2)) UPc o\<^sub>C\<^sub>L (X;(X1;D1)) UPc\<close>
+
+end
